theories/Fundamental.v
@@ -1,8 +1,8 @@
 (** * LogRel.Fundamental: declarative typing implies the logical relation for any generic instance. *)
 From LogRel Require Import Utils Syntax.All GenericTyping DeclarativeTyping LogicalRelation.
-From LogRel.LogicalRelation Require Import Escape Irrelevance Reflexivity Transitivity Weakening Neutral Induction NormalRed.
-From LogRel.LogicalRelation.Introductions Require Import Universe.
-From LogRel.Validity Require Import Validity Irrelevance Properties Conversion Reflexivity SingleSubst Escape.
+From LogRel.LogicalRelation Require Import Properties.
+(* From LogRel.LogicalRelation.Introductions Require Import Universe. *)
+From LogRel.Validity Require Import Validity Irrelevance Properties ValidityTactics.
 From LogRel.Validity.Introductions Require Import Application Universe Pi Lambda Var Nat Empty SimpleArr Sigma Id.
 
 Set Primitive Projections.
@@ -29,7 +29,7 @@ Module FundTy.
     VA : [ Γ ||-v< one > A | VΓ ]
   }.
 
-  Arguments FundTy {_ _ _ _ _ _ _ _ _ _ _ _}.
+  Arguments FundTy {_ _ _ _ _ _ _ _ _ _}.
 End FundTy.
 
 Export FundTy(FundTy,Build_FundTy).
@@ -39,11 +39,9 @@ Module FundTyEq.
     {Γ : context} {A B : term}
   : Type := {
     VΓ : [||-v Γ ];
-    VA : [ Γ ||-v< one > A | VΓ ];
-    VB : [ Γ ||-v< one > B | VΓ ];
-    VAB : [ Γ ||-v< one > A ≅ B | VΓ | VA ]
+    VAB : [ Γ ||-v< one > A ≅ B | VΓ ]
   }.
-  Arguments FundTyEq {_ _ _ _ _ _ _ _ _ _ _ _}.
+  Arguments FundTyEq {_ _ _ _ _ _ _ _ _ _}.
 End FundTyEq.
 
 Export FundTyEq(FundTyEq,Build_FundTyEq).
@@ -56,7 +54,7 @@ Module FundTm.
     VA : [ Γ ||-v< one > A | VΓ ];
     Vt : [ Γ ||-v< one > t : A | VΓ | VA ];
   }.
-  Arguments FundTm {_ _ _ _ _ _ _ _ _ _ _ _}.
+  Arguments FundTm {_ _ _ _ _ _ _ _ _ _}.
 End FundTm.
 
 Export FundTm(FundTm,Build_FundTm).
@@ -69,11 +67,13 @@ Module FundTmEq.
     VA : [ Γ ||-v< one > A | VΓ ];
     Vtu : [ Γ ||-v< one > t ≅ u : A | VΓ | VA ];
   }.
-  Arguments FundTmEq {_ _ _ _ _ _ _ _ _ _ _ _}.
+  Arguments FundTmEq {_ _ _ _ _ _ _ _ _ _}.
 End FundTmEq.
 
 Export FundTmEq(FundTmEq,Build_FundTmEq).
 
+
+(* TODO: Unused ? *)
 Module FundSubst.
   Record FundSubst `{GenericTypingProperties}
     {Γ Δ : context} {wfΓ : [|- Γ]} {σ : nat -> term}
@@ -81,11 +81,12 @@ Module FundSubst.
     VΔ : [||-v Δ ] ;
     Vσ : [VΔ | Γ ||-v σ : Δ | wfΓ] ;
   }.
-  Arguments FundSubst {_ _ _ _ _ _ _ _ _ _ _ _}.
+  Arguments FundSubst {_ _ _ _ _ _ _ _ _ _}.
 End FundSubst.
 
 Export FundSubst(FundSubst,Build_FundSubst).
 
+(* TODO: Unused ? *)
 Module FundSubstConv.
   Record FundSubstConv `{GenericTypingProperties}
     {Γ Δ : context} {wfΓ : [|- Γ]} {σ σ' : nat -> term}
@@ -93,7 +94,7 @@ Module FundSubstConv.
     VΔ : [||-v Δ ] ;
     Veq : [VΔ | Γ ||-v σ ≅ σ' : Δ | wfΓ ] ;
   }.
-  Arguments FundSubstConv {_ _ _ _ _ _ _ _ _ _ _ _}.
+  Arguments FundSubstConv {_ _ _ _ _ _ _ _ _ _}.
 End FundSubstConv.
 
 Export FundSubstConv(FundSubstConv,Build_FundSubstConv).
@@ -110,11 +111,7 @@ Section Fundamental.
   Import DeclarativeTypingData.
 
   Lemma FundConNil : FundCon ε.
-  Proof.
-  unshelve econstructor.
-  + unshelve econstructor; intros; exact unit.
-  + constructor.
-  Qed.
+  Proof. eapply validEmpty. Qed.
 
   Lemma FundConCons (Γ : context) (A : term)
   (fΓ : FundCon Γ) (fA : FundTy Γ A) : FundCon (Γ,, A).
@@ -134,9 +131,7 @@ Section Fundamental.
   Proof.
     destruct fF as [ VΓ VF ]. destruct fG as [ VΓF VG ].
     econstructor.
-    unshelve eapply (PiValid VΓ).
-    - assumption.
-    - now eapply irrelevanceTy.
+    unshelve eapply (PiValid VΓ); irrValid.
   Qed.
 
   Lemma FundTyUniv (Γ : context) (A : term)
@@ -153,7 +148,8 @@ Section Fundamental.
   Proof.
     intros Γ n d FΓ hin.
     unshelve econstructor; tea.
-    + eapply in_ctx_valid in hin as []; now eapply embValidTyOne.
+    + pose proof (in_ctx_valid hin FΓ) as (?&?&?).
+      now eapply lrefl, embValidTyOne.
     + now eapply varnValid.
   Qed.
 
@@ -162,11 +158,8 @@ Section Fundamental.
     FundTm (Γ,, A) U B -> FundTm Γ U (tProd A B).
   Proof.
     intros * [] []; econstructor.
-    eapply PiValidU; irrValid.
-    Unshelve.
-    3: eapply UValid.
-    2: eapply univValid.
-    all:tea.
+    unshelve eapply PiValidU;
+    first [now eapply UValid| now eapply univValid| irrValid | tea].
   Qed.
 
   Lemma FundTmLambda : forall (Γ : context) (A B t : term),
@@ -174,8 +167,8 @@ Section Fundamental.
     FundTm (Γ,, A) B t -> FundTm Γ (tProd A B) (tLambda A t).
   Proof.
     intros * [] []; econstructor.
-    eapply lamValid; irrValid.
-    Unshelve. all: irrValid.
+    unshelve (eapply lamValid; irrValid); irrValid.
+    Unshelve. tea.
   Qed.
 
   Lemma FundTmApp : forall (Γ : context) (f a A B : term),
@@ -192,8 +185,8 @@ Section Fundamental.
     FundTyEq Γ A B -> FundTm Γ B t.
   Proof.
     intros * [] []; econstructor.
-    eapply conv; irrValid.
-    Unshelve. all: tea.
+    irrValid.
+    Unshelve. tea. irrValid.
   Qed.
 
   Lemma FundTyEqPiCong : forall (Γ : context) (A B C D : term),
@@ -202,9 +195,7 @@ Section Fundamental.
     FundTyEq (Γ,, A) C D -> FundTyEq Γ (tProd A C) (tProd B D).
   Proof.
     intros * [] [] []; econstructor.
-    - eapply PiValid. eapply irrelevanceLift; tea; irrValid.
-    - eapply PiCong. 1: eapply irrelevanceLift; tea.
-      all: irrValid.
+    eapply PiValid. irrValid.
     Unshelve. all: tea; irrValid.
   Qed.
 
@@ -218,7 +209,7 @@ Section Fundamental.
     FundTyEq Γ A B -> FundTyEq Γ B A.
   Proof.
     intros * [];  unshelve econstructor; tea.
-    now eapply symValidTyEq.
+    irrValid.
   Qed.
 
   Lemma FundTyEqTrans : forall (Γ : context) (A B C : term),
@@ -226,20 +217,14 @@ Section Fundamental.
     FundTyEq Γ B C ->
     FundTyEq Γ A C.
   Proof.
-    intros * [] []; unshelve econstructor; tea. 1:irrValid.
-    eapply transValidTyEq; irrValid.
-    Unshelve. 2:tea.
+    intros * [] []; unshelve econstructor; tea; irrValid.
   Qed.
 
   Lemma FundTyEqUniv : forall (Γ : context) (A B : term),
     FundTmEq Γ U A B -> FundTyEq Γ A B.
   Proof.
     intros * [?? VAB].
-    pose proof (lreflValidTm _ VAB).
-    pose proof (ureflValidTm VAB).
-    unshelve econstructor; tea.
-    1,2: now eapply univValid.
-    now eapply univEqValid.
+    unshelve econstructor; tea; now eapply univValid.
   Qed.
 
   Lemma FundTmEqBRed : forall (Γ : context) (a t A B : term),
@@ -248,8 +233,8 @@ Section Fundamental.
     FundTm Γ A a -> FundTmEq Γ B[a..] (tApp (tLambda A t) a) t[a..].
   Proof.
     intros * [] [] []; econstructor.
-    - unshelve epose (betaValid VA _ _ _). 2,5-7:irrValid.
-      Unshelve. 1:tea. eapply substS; tea; irrValid.
+    eapply betaValid; irrValid.
+    Unshelve. all: cycle 2; irrValid.
   Qed.
 
   Lemma FundTmEqPiCong : forall (Γ : context) (A B C D : term),
@@ -259,20 +244,10 @@ Section Fundamental.
     FundTmEq Γ U (tProd A C) (tProd B D).
   Proof.
     intros * [] [] [].
-    assert (VA' : [Γ ||-v<one> A | VΓ]) by now eapply univValid.
-    assert (VAB : [Γ ||-v<one> A ≅ B | VΓ | VA']) by (eapply univEqValid; irrValid).
-    pose proof (ureflValidTy VAB).
-    opector; tea.
-    - eapply UValid.
-    - unshelve epose (PiCongTm _ _ _ _ _ _ _ _ _ _ _).
-      17: irrValid.
-      2: tea.
-      2,3,8: eapply irrelevanceTmEq; tea; first [now eapply lreflValidTm| now eapply ureflValidTm].
-      all: try (irrValid + eapply irrelevanceTmEq ;now eapply ureflValidTm).
-      + eapply UValid.
-      + eapply irrelevanceTmLift; tea; now eapply irrelevanceTmEq, ureflValidTm.
-      Unshelve.
-      all: try irrValid.
+    (* assert (VA' : [Γ ||-v<one> A | VΓ]) by now eapply univValid. *)
+    assert (VAB : [Γ ||-v<one> A ≅ B | VΓ ]) by now unshelve (eapply univValid; irrValid).
+    econstructor. eapply PiCongTm; tea; irrValid.
+    Unshelve. all: irrValid.
   Qed.
 
   Lemma FundTmEqAppCong : forall (Γ : context) (a b f g A B : term),
@@ -280,9 +255,13 @@ Section Fundamental.
     FundTmEq Γ A a b ->
     FundTmEq Γ B[a..] (tApp f a) (tApp g b).
   Proof.
-    intros * [] []; econstructor.
-    eapply appcongValid; first [irrValid | now eapply ureflValidTm].
-    Unshelve. 1: irrValid. now eapply lreflValidTm.
+    intros * [? VΠ] [?? Vab]; pose (VB := validΠcod VΠ).
+    opector; tea.
+    1: unshelve (eapply lrefl, substS; tea; irrValid); irrValid.
+    unshelve epose proof (appcongValid (a:=a) (b:=b) Vtu _); [irrValid|].
+    (* Completeness issue with irrValid... *)
+    (* irrValid. *)
+    eapply irrValidTm; tea.
   Qed.
 
   Lemma FundTmEqLambdaCong : forall (Γ : context) (t u A A' A'' B : term),
@@ -291,21 +270,15 @@ Section Fundamental.
     FundTyEq Γ A A'' ->
     FundTmEq (Γ,, A) B t u -> FundTmEq Γ (tProd A B) (tLambda A' t) (tLambda A'' u).
   Proof.
-    intros * [VΓ] [? ? VA'] [? ? VA''] [].
+    intros * [VΓ] [? VA'] [? VA''] [].
+    assert (VAeq : [_ ||-v<one> A' ≅ A'' | VΓ]) by irrValid.
+    pose proof (validSnoc _ VA'); pose proof (validSnoc _ VA'').
+    assert (VB : [_ ||-v<one> B | validSnoc VΓ VAeq]) by irrValid.
+    assert (Vteq : [_ ||-v<one> t ≅ u : _ | _ | VB]) by irrValid.
+    pose proof (lamCongValid VAeq  VB Vteq).
     econstructor.
-    eapply conv.
-    2:{ eapply lamCongValid; tea.
-      + unshelve (eapply transValidTyEq; tea; eapply symValidTyEq); try irrValid.
-      + now eapply convCtx1.
-      + eapply convEqCtx1; tea; now eapply reflValidTy.
-      + now eapply convTmEqCtx1.
-    }
-    unshelve (eapply PiCong; [|eapply symValidTyEq|eapply reflValidTy]; irrValid); try irrValid.
-    Unshelve.
-    5: tea.
-    3: now eapply convCtx1.
-    2: irrValid.
-    unshelve eapply PiValid; irrValid.
+    eapply irrValidTm; tea; eapply PiValid; irrValid.
+    Unshelve.  all: first [assumption|unshelve eapply PiValid; irrValid| irrValid].
   Qed.
 
   Lemma FundTmEqFunEta : forall (Γ : context) (f A B : term),
@@ -315,32 +288,9 @@ Section Fundamental.
   eapply etaValid; irrValid.
   Unshelve.
   + tea.
-  + now eapply PiValidDom.
-  + now eapply PiValidCod.
+  + now eapply validΠdom.
+  + now eapply validΠcod.
   Qed.
-
-  (* Lemma FundTmEqFunExt : forall (Γ : context) (f g A B : term),
-    FundTy Γ A ->
-    FundTm Γ (tProd A B) f ->
-    FundTm Γ (tProd A B) g ->
-    FundTmEq (Γ,, A) B (tApp (f⟨↑⟩) (tRel 0)) (tApp (g⟨↑⟩) (tRel 0)) ->
-    FundTmEq Γ (tProd A B) f g.
-  Proof.
-    intros * [] [VΓ0 VA0] [] [].
-    assert [Γ ||-v< one > g : tProd A B | VΓ0 | VA0].
-    1:{
-      eapply conv.
-      2: irrValid.
-      eapply symValidTyEq. eapply PiCong.
-      eapply irrelevanceLift.
-      1,3,4: eapply reflValidTy.
-      irrValid.
-    }
-    econstructor.
-    3: eapply etaeqValid.
-    5: do 2 rewrite wk1_ren_on.
-    Unshelve. all: irrValid.
-  Qed. *)
 
   Lemma FundTmEqRefl : forall (Γ : context) (t A : term),
     FundTm Γ A t ->
@@ -353,7 +303,7 @@ Section Fundamental.
     FundTmEq Γ A t t' ->
     FundTmEq Γ A t' t.
   Proof.
-    intros * []; econstructor; tea; now eapply symValidTmEq.
+    intros * []; unshelve econstructor; tea; irrValid.
   Qed.
 
   Lemma FundTmEqTrans : forall (Γ : context) (t t' t'' A : term),
@@ -361,9 +311,7 @@ Section Fundamental.
     FundTmEq Γ A t' t'' ->
     FundTmEq Γ A t t''.
   Proof.
-    intros * [] []; econstructor; tea.
-    eapply transValidTmEq; irrValid.
-    Unshelve. all: tea.
+    intros * [] []; unshelve econstructor; irrValid.
   Qed.
 
   Lemma FundTmEqConv : forall (Γ : context) (t t' A B : term),
@@ -371,9 +319,7 @@ Section Fundamental.
     FundTyEq Γ A B ->
     FundTmEq Γ B t t'.
   Proof.
-    intros * [] []; econstructor.
-    eapply conv; irrValid.
-    Unshelve. all: irrValid.
+    intros * [] []; unshelve econstructor; irrValid.
   Qed.
 
   Lemma FundTyNat : forall Γ : context, FundCon Γ -> FundTy Γ tNat.
@@ -396,9 +342,7 @@ Section Fundamental.
   Lemma FundTmSucc : forall (Γ : context) (n : term),
     FundTm Γ tNat n -> FundTm Γ tNat (tSucc n).
   Proof.
-    intros * []; unshelve econstructor; tea.
-    eapply irrelevanceTm; eapply succValid; irrValid.
-    Unshelve. tea.
+    intros * []; unshelve econstructor; tea; now eapply succValid'.
   Qed.
 
   Lemma FundTmNatElim : forall (Γ : context) (P hz hs n : term),
@@ -409,8 +353,7 @@ Section Fundamental.
   Proof.
     intros * [] [] [] []; unshelve econstructor; tea.
     2: eapply natElimValid; irrValid.
-    Unshelve.
-    2,3: irrValid.
+    Unshelve. all: irrValid.
   Qed.
 
   Lemma FundTyEmpty : forall Γ : context, FundCon Γ -> FundTy Γ tEmpty.
@@ -430,15 +373,13 @@ Section Fundamental.
   Proof.
     intros * [] []; unshelve econstructor; tea.
     2: eapply emptyElimValid; irrValid.
-    Unshelve. 2,3: irrValid.
+    Unshelve. all: irrValid.
   Qed.
 
   Lemma FundTmEqSuccCong : forall (Γ : context) (n n' : term),
     FundTmEq Γ tNat n n' -> FundTmEq Γ tNat (tSucc n) (tSucc n').
   Proof.
-    intros * []; unshelve econstructor; tea.
-    eapply irrelevanceTmEq; eapply succcongValid; irrValid.
-    Unshelve. all: tea.
+    intros * []; unshelve econstructor; tea; now eapply succValid'.
   Qed.
 
   Lemma FundTmEqNatElimCong : forall (Γ : context)
@@ -449,10 +390,11 @@ Section Fundamental.
     FundTmEq Γ tNat n n' ->
     FundTmEq Γ P[n..] (tNatElim P hz hs n) (tNatElim P' hz' hs' n').
   Proof.
-    intros * [? VP0 VP0'] [VΓ0] [] []; unshelve econstructor.
-    3:eapply natElimCongValid; try irrValid.
-    tea.
-    Unshelve. all: irrValid.
+    intros * [? VP0] [VΓ0] [] []; opector; tea.
+    1: unshelve (eapply lrefl, substS; irrValid); eapply natValid.
+    eapply irrValidTm.
+    2: unshelve (eapply natElimCongValid; try irrValid).
+    Unshelve.  all: first [exact Γ| exact one| eassumption| irrValid].
   Qed.
 
   Lemma FundTmEqNatElimZero : forall (Γ : context) (P hz hs : term),
@@ -463,7 +405,6 @@ Section Fundamental.
   Proof.
     intros * [] [] []; unshelve econstructor; tea.
     2: eapply natElimZeroValid; try irrValid.
-    now eapply reflValidTy.
     Unshelve. irrValid.
   Qed.
 
@@ -477,7 +418,6 @@ Section Fundamental.
   Proof.
     intros * [] [] [] []; unshelve econstructor; tea.
     2: eapply natElimSuccValid; try irrValid.
-    now eapply reflValidTy.
     Unshelve. all: irrValid.
   Qed.
 
@@ -487,9 +427,12 @@ Section Fundamental.
     FundTmEq Γ tEmpty n n' ->
     FundTmEq Γ P[n..] (tEmptyElim P n) (tEmptyElim P' n').
   Proof.
-    intros * [? VP0 VP0'] [VΓ0]; unshelve econstructor; tea.
+    intros * [? VP0 ] [VΓ0]; opector; tea.
+    1: unshelve (eapply lrefl, substS; irrValid); eapply emptyValid.
+    eapply irrValidTm.
     2: eapply emptyElimCongValid; irrValid.
-    Unshelve. all: irrValid.
+    tea.
+    Unshelve.  all: first [exact Γ| exact one| eassumption| irrValid].
   Qed.
 
   Lemma FundTySig : forall (Γ : context) (A B : term),
@@ -503,12 +446,10 @@ Section Fundamental.
     FundTm Γ U A ->
     FundTm (Γ,, A) U B -> FundTm Γ U (tSig A B).
   Proof.
-    intros * [] []; unshelve econstructor; tea.
-    unshelve epose (SigCongValidU (F:=A) (G:=B) _ _ ).
-    6,7,8: irrValid.
-    + tea.
-    + now eapply univValid.
-    + irrValid.
+    intros * [] []; unshelve econstructor.
+    3:eapply SigCongValidU; irrValid.
+    tea.
+    Unshelve. 1: now eapply univValid. irrValid.
   Qed.
 
   Lemma FundTmPair : forall (Γ : context) (A B a b : term),
@@ -518,28 +459,26 @@ Section Fundamental.
     FundTm Γ B[a..] b -> FundTm Γ (tSig A B) (tPair A B a b).
   Proof.
     intros * [] [] [] []; unshelve econstructor.
-    3: unshelve eapply pairValid; irrValid.
+    3: eapply pairValid; irrValid.
     tea.
+    Unshelve. 2-4: irrValid.
   Qed.
 
   Lemma FundTmFst : forall (Γ : context) (A B p : term),
     FundTm Γ (tSig A B) p -> FundTm Γ A (tFst p).
   Proof.
     intros * []; unshelve econstructor.
-    3: unshelve eapply fstValid.
-    5: irrValid.
-    2: now eapply domSigValid.
-    now eapply codSigValid.
+    3: eapply fstValid; try irrValid.
+    2: now eapply validΣdom.
+    Unshelve. 2: eapply validΣcod.
   Qed.
 
   Lemma FundTmSnd : forall (Γ : context) (A B p : term),
     FundTm Γ (tSig A B) p -> FundTm Γ B[(tFst p)..] (tSnd p).
   Proof.
-    intros * []; unshelve econstructor.
-    3: unshelve eapply sndValid.
-    5: irrValid.
-    2: now eapply domSigValid.
-    now eapply codSigValid.
+    intros * []; econstructor.
+    unshelve eapply sndValid; cycle 2;
+    try first [now eapply validΣdom | now eapply validΣcod| irrValid].
   Qed.
 
   Lemma FundTyEqSigCong : forall (Γ : context) (A B C D : term),
@@ -549,10 +488,8 @@ Section Fundamental.
   Proof.
     intros * [] [] [].
     unshelve econstructor.
-    4: eapply SigCong; tea; try irrValid.
-    2: eapply irrelevanceLift; irrValid.
-    eapply SigValid; eapply irrelevanceLift; irrValid.
-    Unshelve. all: irrValid.
+    2: eapply SigValid; tea; try irrValid.
+    tea. Unshelve. tea.
   Qed.
 
   Lemma FundTmEqSigCong :forall (Γ : context) (A A' B B' : term),
@@ -562,7 +499,7 @@ Section Fundamental.
   Proof.
     intros * [] [] []; unshelve econstructor.
     3: eapply SigCongValidU ; tea; try irrValid.
-    1: tea.
+    tea.
     Unshelve.
     + unshelve (eapply univValid; irrValid); irrValid.
     + irrValid.
@@ -577,22 +514,21 @@ Section Fundamental.
     FundTmEq Γ A a a' ->
     FundTmEq Γ B[a..] b b' -> FundTmEq Γ (tSig A B) (tPair A' B' a b) (tPair A'' B'' a' b').
   Proof.
-    intros * [VΓ VA] [?? VA'] [] [] [] [] [].
-    assert [Γ ,, A' ||-v<one> B' | validSnoc _ VA'].
-    1:{ eapply convCtx1; tea. }
+    intros * [VΓ VA] [? VA'] [? VA''] [? VB] [? VB''] [?? Va] [?? Vb].
+    assert (VAeq : [_ ||-v<one> A' ≅ A'' | VΓ]) by irrValid.
+    pose proof (validSnoc _ VA'); pose proof (validSnoc _ VA'').
+    assert (VBeq0 : [_ ||-v<one> B ≅ B' | validSnoc VΓ VAeq]) by irrValid.
+    assert (VBeq1 : [_ ||-v<one> B ≅ B'' | validSnoc VΓ VAeq]) by irrValid.
+    assert (VBeq2 : [_ ||-v<one> B' ≅ B'' | validSnoc VΓ VAeq]) by irrValid.
+    assert (Vaeq : [_ ||-v<one> a ≅ a' : _ | _ | VAeq]) by irrValid.
+    pose proof (substS VBeq0 Vaeq).
+    pose proof (substS VBeq1 Vaeq).
+    pose (VBaeq := substS VBeq2 Vaeq).
+    assert (Vbeq : [_ ||-v<one> b ≅ b' : _ | _ | VBaeq]) by irrValid.
+    epose (pairCongValid _ _ _ Vaeq Vbeq).
     econstructor.
-    eapply conv; cycle 1.
-    - eapply pairCongValid.
-      + eapply transValidTyEq; tea; eapply symValidTyEq; irrValid.
-      + eapply convEqCtx1; tea; eapply transValidTyEq; tea.
-        eapply symValidTyEq; irrValid.
-      + eapply conv; [eapply substSEq; tea|]; irrValid.
-    - eapply symValidTyEq; eapply SigCong; try irrValid.
-    Unshelve.
-      all: try irrValid.
-      + unshelve eapply SigValid; irrValid.
-      + unshelve (eapply conv; tea; irrValid); irrValid.
-      + eapply lreflValidTm; irrValid.
+    eapply irrValidTm; tea; unshelve eapply SigValid; irrValid.
+    Unshelve. 1,3: tea. unshelve eapply SigValid; irrValid.
   Qed.
 
   Lemma FundTmEqSigEta : forall (Γ : context) (A B p : term),
@@ -602,8 +538,8 @@ Section Fundamental.
   eapply sigEtaValid; irrValid.
   Unshelve.
   + tea.
-  + now eapply domSigValid.
-  + now eapply codSigValid.
+  + now eapply validΣdom.
+  + now eapply validΣcod.
   Qed.
 
   Lemma FundTmEqFstCong : forall (Γ : context) (A B p p' : term),
@@ -611,8 +547,8 @@ Section Fundamental.
   Proof.
     intros * []; unshelve econstructor.
     3: eapply fstValid; irrValid.
-    2: now eapply domSigValid.
-    Unshelve. all: now eapply codSigValid.
+    2: now eapply validΣdom.
+    Unshelve. 2: eapply validΣcod.
   Qed.
 
   Lemma FundTmEqFstBeta : forall (Γ : context) (A B a b : term),
@@ -632,14 +568,13 @@ Section Fundamental.
   Lemma FundTmEqSndCong : forall (Γ : context) (A B p p' : term),
     FundTmEq Γ (tSig A B) p p' -> FundTmEq Γ B[(tFst p)..] (tSnd p) (tSnd p').
   Proof.
-    intros * []; unshelve econstructor.
-    3: eapply sndValid; irrValid.
-    1: tea.
-    Unshelve.
-      2: now eapply domSigValid.
-      1: now eapply codSigValid.
-      irrValid.
+    intros * [? VΣ].
+    assert (Vp : [_ ||-v<one> p ≅ p' : _ | _ | SigValid _ (validΣdom VΣ) (validΣcod VΣ)]) by irrValid.
+    pose (t := sndValid _ _ _ Vp); set (VBfst := substS _ _) in t.
+    econstructor. eapply irrValidTm; tea; irrValid.
+    Unshelve. all: first [eassumption| irrValid].
   Qed.
+
 
   Lemma FundTmEqSndBeta : forall (Γ : context) (A B a b : term),
     FundTy Γ A ->
@@ -648,10 +583,13 @@ Section Fundamental.
     FundTm Γ B[a..] b ->
     FundTmEq Γ B[(tFst (tPair A B a b))..] (tSnd (tPair A B a b)) b.
   Proof.
-    intros * [] [] [] []; unshelve econstructor.
-    3: eapply pairSndValid.
-    1: tea.
-    Unshelve. all: irrValid.
+    intros * [] [] [] [].
+    unshelve epose (Vsnd := pairSndValid (B:=B) (a:=a) (b:=b) _ VA _ _ _).
+    1-3: irrValid.
+    ltac2:(HoistLetIn.hoist_let_in @Vsnd).
+    unshelve econstructor; [tea| irrValid|].
+    unshelve eapply irrValidTm, pairSndValid.
+    9: tea. 2: tea. 2-4: irrValid.
   Qed.
 
   Lemma FundTyId : forall (Γ : context) (A x y : term),
@@ -669,7 +607,7 @@ Section Fundamental.
       intros * [] [] [].
       unshelve econstructor; tea.
       1: eapply UValid.
-      unshelve eapply IdTmValid; cycle 1; try irrValid; tea.
+      unshelve eapply IdValidU ; cycle 1; first [exact one| irrValid].
   Qed.
 
   Lemma FundTmRefl : forall (Γ : context) (A x : term),
@@ -687,10 +625,11 @@ Section Fundamental.
     FundTm Γ P[tRefl A x .: x..] hr ->
     FundTm Γ A y -> FundTm Γ (tId A x y) e -> FundTm Γ P[e .: y..] (tIdElim A x P hr y e).
   Proof.
-    intros * [] [] [] [] [] []; unshelve econstructor.
-    3: unshelve eapply IdElimValid; try irrValid.
-    2,3: eapply reflValidTy.
-    tea.
+    intros * [] [?? Vx] [? VP] [?? Vhr] [?? Vy] [?? Ve].
+    unshelve epose proof (Velim := IdElimValid (hr:=hr) (hr':=hr) _ _ _ _ VP _ _ _ Ve).
+    1-4: irrValid.
+    ltac2:(HoistLetIn.hoist_let_in @Velim).
+    now unshelve econstructor.
   Qed.
 
   Lemma FundTyEqId : forall (Γ : context) (A A' x x' y y' : term),
@@ -699,9 +638,7 @@ Section Fundamental.
   Proof.
     intros * [] [] [].
     unshelve econstructor; tea.
-    3: eapply IdCongValid; irrValid.
-    1,2: eapply IdValid; try irrValid.
-    1,2: eapply ureflValidTm, conv; tea; try irrValid.
+    eapply IdValid; irrValid.
     Unshelve. all: irrValid.
   Qed.
 
@@ -710,18 +647,17 @@ Section Fundamental.
     FundTmEq Γ A x x' -> FundTmEq Γ A y y' -> FundTmEq Γ U (tId A x y) (tId A' x' y').
   Proof.
     intros * [] [] []; unshelve econstructor.
-    3: eapply IdTmCongValid; try irrValid; tea.
-    1: tea.
-    Unshelve. all: first [eapply UValid| irrValid | tea].
+    3: unshelve (eapply IdValidU; first [irrValid | tea]).
+    all: first [exact one | eassumption | irrValid].
   Qed.
 
   Lemma FundTmEqReflCong : forall (Γ : context) (A A' x x' : term),
     FundTyEq Γ A A' -> FundTmEq Γ A x x' -> FundTmEq Γ (tId A x x) (tRefl A x) (tRefl A' x').
   Proof.
-    intros * [] []; unshelve econstructor.
-    3: eapply reflCongValid; tea; irrValid.
+    intros * [] []; unshelve econstructor; tea.
+    2: eapply reflValid; try irrValid.
     eapply IdValid; irrValid.
-    Unshelve. tea.
+    Unshelve. all: irrValid.
   Qed.
 
   Lemma FundTmEqIdElimCong : forall (Γ : context) (A A' x x' P P' hr hr' y y' e e' : term),
@@ -734,13 +670,23 @@ Section Fundamental.
     FundTmEq Γ A y y' ->
     FundTmEq Γ (tId A x y) e e' -> FundTmEq Γ P[e .: y..] (tIdElim A x P hr y e) (tIdElim A' x' P' hr' y' e').
   Proof.
-    intros * [] [] [] [] [] [] [] [].
-    econstructor.
-    eapply IdElimValid; tea; irrValid.
-    Unshelve.
-    3: unshelve (eapply IdValid; irrValid); irrValid.
-    all: irrValid.
+    intros * [] [?? Vx] [? VA'] [?? Vx'] [? VP] [?? Vhr] [?? Vy] [?? Ve].
+    unshelve epose proof (VΓext :=idElimMotiveCtxEq (x:=x) (x':=x') _ VA' _); [irrValid|].
+    unfold idElimMotiveCtxEqStmt in *.
+    assert (VPext : [ _ ||-v<one> P ≅ P' | VΓext]) by irrValid.
+    unshelve epose proof (VId := IdValid (x:=x) (x':=x') (y:=y) (y':=y') _ VA' _ _).
+    1-2: irrValid.
+    assert (Ve' : [_ ||-v<one> e ≅ e' : _ | _ | VId]) by irrValid.
+    unshelve epose proof (Velim := IdElimValid (hr:=hr) (hr':=hr') _ _ _ _ VPext _ _ VId Ve').
+    1-4: irrValid.
+    ltac2:(HoistLetIn.hoist_let_in @Velim).
+    unshelve econstructor; tea.
+    1: irrValid.
+    eapply irrValidTm; tea.
+    irrValid.
+    Unshelve. tea.
   Qed.
+
 
   Lemma FundTmEqIdElimRefl : forall (Γ : context) (A x P hr y A' z : term),
     FundTy Γ A ->
@@ -754,21 +700,24 @@ Section Fundamental.
     FundTmEq Γ A x y ->
     FundTmEq Γ A x z -> FundTmEq Γ P[tRefl A' z .: y..] (tIdElim A x P hr y (tRefl A' z)) hr.
   Proof.
-    intros * [] [] [] [] [] [] [] [] [] [].
+    intros * [] [] [] [] [] [] [] [? VAA'] [] [].
+    pose (VA' := urefl VAA').
+    assert [_ ||-v<one> x ≅ z : _ | _ | VA'] by irrValid.
+    assert [_ ||-v<one> y ≅ z : _ | _ | VA'] by irrValid.
     econstructor.
-    eapply IdElimReflValid; tea; try irrValid.
-    Unshelve. all: try irrValid.
+    eapply IdElimReflValid; irrValid.
+    Unshelve.
+      1: tea. 1,2: irrValid.
+      + unshelve eapply idElimMotiveCtxEq; tea; first [exact one |irrValid].
+      + irrValid.
       + unshelve (eapply IdValid; irrValid); irrValid.
-      + assert (VId : [Γ ||-v<one> tId A x y | VΓ]) by (unshelve (eapply IdValid; irrValid); irrValid).
-        assert [_ ||-v<one> y ≅ z : _ | _ | VA].
-        1: eapply transValidTmEq; [eapply symValidTmEq|]; irrValid.
-        assert [Γ ||-v<one> tId A x y ≅ tId A' z z | _ | VId ].
-        1: eapply IdCongValid; irrValid.
-        eapply conv; [|eapply reflValid, ureflValidTm, conv; irrValid].
-        eapply symValidTyEq; irrValid.
-        Unshelve.
-          2: unshelve eapply ureflValidTy.
-          all: try irrValid.
+      + eapply irrValidTm.
+        2: eapply reflValid, urefl; tea.
+        1: eapply IdValid; irrValid.
+        exact one.
+    Unshelve.
+      2: tea. 3: irrValid.
+      2:eapply IdValid; now symmetry.
   Qed.
 
 
@@ -854,16 +803,12 @@ Lemma Fundamental : (forall Γ : context, [ |-[ de ] Γ ] -> FundCon (ta := ta) 
     - inversion HΔ as [|?? HΔ' HA] ; subst ; clear HΔ ; refold.
       destruct IH ; tea.
       apply Fundamental in Hσ0 as [?? Hσ0].
-      cbn in *.
-      eapply reducibleTmEq in Hσ0.
       eapply Fundamental in HA as [].
       unshelve econstructor.
       1: now eapply validSnoc.
       unshelve econstructor.
       + now eapply irrelevanceSubst.
-      + cbn; irrelevance0.
-        2: eassumption.
-        reflexivity.
+      + now eapply redValidTm'.
   Qed.
 
   Corollary Fundamental_subst_conv Γ Δ σ σ' (wfΓ : [|-[ta] Γ ]) :
@@ -878,15 +823,13 @@ Lemma Fundamental : (forall Γ : context, [ |-[ de ] Γ ] -> FundCon (ta := ta) 
       all: now econstructor.
     - inversion HΔ as [|?? HΔ' HA] ; subst ; clear HΔ ; refold.
       destruct IH ; tea.
-      apply Fundamental in Hσ0 as [?? Ηστ] ; cbn in *.
+      apply Fundamental in Hσ0 as [?? Hστ] ; cbn in *.
       eapply Fundamental in HA as [? HA].
       unshelve econstructor.
       + now eapply validSnoc.
       + unshelve econstructor.
-        1: now irrValid.
-        cbn.
-        irrelevanceRefl.
-        now eapply reducibleTmEq.
+        1: now eapply irrelevanceSubst.
+        eapply irrLREq; [reflexivity| now eapply redValidTm].
   Qed.
 
 End Fundamental.
