theories/LogicalRelation/Introductions/Id.v
@@ -25,50 +25,6 @@ Section IdRed.
       [Γ ||-<l> tId A t u ≅ tId A' t' u'].
   Proof. intros; apply LRId'; now eapply IdRed0. Defined.
 
-  (* Lemma IdRedTy_inv {Γ l A t u B} (RIA : [Γ ||-Id<l> tId A t u]) :
-    [× A = RIA.(IdRedTy.ty), t = RIA.(IdRedTy.lhs) & u = RIA.(IdRedTy.rhs)].
-  Proof.
-    pose proof (redtywf_whnf RIA.(IdRedTy.red) whnf_tId) as e; injection e; now split.
-  Qed.
-
-  Lemma IdCongRed {Γ l A A' t t' u u'}
-    (RA : [Γ ||-<l> A])
-    (RIA : [Γ ||-<l> tId A t u]) :
-    [Γ |- tId A' t' u'] ->
-    [RA | _ ||- _ ≅ A'] ->
-    [RA | _ ||- t ≅ t' : _] ->
-    [RA | _ ||- u ≅ u' : _] ->
-    [RIA | _ ||- _ ≅ tId A' t' u'].
-  Proof.
-    intros.
-    enough [LRId' (invLRId RIA) | _ ||- _ ≅ tId A' t' u'] by irrelevance.
-    pose proof (IdRedTy_inv (invLRId (RIA))) as [ety elhs erhs].
-    econstructor.
-    + now eapply redtywf_refl.
-    + unfold_id_outTy; rewrite <- ety, <- elhs, <- erhs; eapply convty_Id; now escape.
-    + irrelevance.
-    + cbn; rewrite <- elhs; irrelevance.
-    + cbn; rewrite <- erhs; irrelevance.
-  Qed. *)
-
-  (* Lemma IdRedU@{i j k l} {Γ l A t u}
-      (RU : [LogRel@{i j k l} l | Γ ||- U])
-      (RU' := invLRU RU)
-      (RA : [LogRel@{i j k l} (URedTy.level RU') | Γ ||- A]) :
-      [RU | Γ ||- A ≅ A' : U] ->
-      [RA | Γ ||- t ≅ t': _] ->
-      [RA | Γ ||- u ≅: _] ->
-      [RU | Γ ||- tId A t u : U].
-  Proof.
-    intros RAU Rt Ru.
-    enough [LRU_ RU' | _ ||- tId A t u : U] by irrelevance.
-    econstructor.
-    (* - eapply redtmwf_refl; escape; now eapply ty_Id. *)
-    - constructor.
-    - eapply convtm_Id; eapply escapeEq + eapply escapeEqTerm; now eapply reflLRTmEq + eapply reflLRTyEq.
-    - eapply RedTyRecBwd. eapply IdRed; irrelevanceCum.
-    Unshelve. irrelevanceCum.
-  Qed. *)
 
   Lemma IdCongRedU@{i j k l} {Γ l A A' t t' u u'}
       (RU : [LogRel@{i j k l} l | Γ ||- U ≅ U])
@@ -92,32 +48,7 @@ Section IdRed.
   Qed.
 
 
-
-(* Lemma reflRed {Γ l A x} (RA : [Γ ||-<l> A]) (Rx : [RA | _ ||- x : _]) (RIA : [Γ ||-<l> tId A x x]) :
-  [RIA | _ ||- tRefl A x : _].
-Proof.
-  set (RIA' := invLRId RIA).
-  enough [LRId' RIA' | _ ||- tRefl A x : _] by irrelevance.
-  pose proof (IdRedTy_inv RIA') as [eA ex ex'].
-  assert (e : tId (IdRedTy.ty RIA') (IdRedTy.lhs RIA') (IdRedTy.rhs RIA') = tId A x x).
-  1: f_equal; now symmetry.
-  econstructor; unfold_id_outTy; cbn; rewrite ?e.
-  + eapply redtmwf_refl; eapply ty_refl; now escape.
-  + eapply convtm_refl; [eapply escapeEq; eapply reflLRTyEq|eapply escapeEqTerm; now eapply reflLRTmEq].
-  + constructor; cbn.
-    1,2: now escape.
-    all: irrelevance0; tea.
-    1: eapply reflLRTyEq.
-    * rewrite <- ex; now eapply reflLRTmEq.
-    * rewrite <- ex'; now eapply reflLRTmEq.
-  Unshelve.  all: tea.
-Qed.
-
-Lemma reflRed' {Γ l A x} (RA : [Γ ||-<l> A]) (Rx : [RA | _ ||- x : _])
-  (RIA := IdRed RA Rx Rx): [RIA | _ ||- tRefl A x : _].
-Proof. now eapply reflRed. Qed. *)
-
-Lemma reflCongRed {Γ l A A0 A' B x x'}
+Lemma reflCongRed0 {Γ l A A0 A' B x x'}
   (RA : [Γ ||-<l> A ≅ A0])
   (wfA' : [Γ |- A'])
   (eqA : [Γ |- A ≅ A'])
@@ -140,7 +71,16 @@ Proof.
   all: first [now eapply irrLREq| now eapply lrefl, irrLREq].
 Qed.
 
+Lemma reflCongRed {Γ l A A' x x'}
+  (RA : [Γ ||-<l> A ≅ A'])
+  (Rxx : [RA | _ ||- x ≅ x' : _])
+  (RIA : [Γ ||-<l> tId A x x ≅ tId A' x' x']) :
+  [RIA | _ ||- tRefl A x ≅ tRefl A' x' : _].
+Proof.
+  escape; now eapply reflCongRed0.
+Qed.
 
+(* Unused ? *)
 Lemma reflCongRed' {Γ l A Al Ar x xl xr}
   (RA : [Γ ||-<l> A])
   (wtyAl : [Γ |- Al])
@@ -151,80 +91,73 @@ Lemma reflCongRed' {Γ l A Al Ar x xl xr}
   (Rxxr : [RA | _ ||- x ≅ xr : _])
   (RIA : [Γ ||-<l> tId A x x]) :
   [RIA | _ ||- tRefl Al xl ≅ tRefl Ar xr : _].
-Proof. etransitivity; [symmetry|]; now eapply (reflCongRed RA), irrLR. Qed.
+Proof. etransitivity; [symmetry|]; now eapply (reflCongRed0 RA), irrLR. Qed.
 
 Lemma idElimPropCongRed {Γ l A A' x x' P P' hr hr' y y' e e'}
-  (RA : [Γ ||-<l> A])
-  (RA' : [Γ ||-<l> A'])
-  (wtyA' := escape RA')
-  (convtyAA' : [Γ |- A ≅ A' ])
+  (RA : [Γ ||-<l> A ≅ A'])
   (Rxx' : [RA | _ ||- x ≅ x' : _])
-  (RIAxx : [Γ ||-<l> tId A x x])
+  (RIAxx : [Γ ||-<l> tId A x x ≅ tId A' x' x'])
   (RP0 : [Γ ,, A ,, tId A⟨@wk1 Γ A⟩ x⟨@wk1 Γ A⟩ (tRel 0) |- P])
   (RP0' : [Γ ,, A' ,, tId A'⟨@wk1 Γ A'⟩ x'⟨@wk1 Γ A'⟩ (tRel 0) |- P'])
   (RPP0 : [Γ ,, A ,, tId A⟨@wk1 Γ A⟩ x⟨@wk1 Γ A⟩ (tRel 0) |- P ≅ P'])
   (RP : forall {y y' e e'}
     (Ryy' : [RA | _ ||- y ≅ y' : _])
-    {RIAxy : [Γ ||-<l> tId A x y]}
+    {RIAxy : [Γ ||-<l> tId A x y ≅ tId A' x' y']}
     (Ree' : [ RIAxy | _ ||- e ≅ e' : _]),
     [Γ ||-<l> P[e .: y..] ≅ P'[e' .: y'..]])
-  (Rrfl := (reflCongRed RA wtyA' convtyAA' Rxx' RIAxx))
+  (Rrfl := (reflCongRed RA Rxx' RIAxx))
   (Rhrhr' : [RP Rxx' Rrfl | _ ||- hr ≅ hr' : _])
   (Ryy' : [RA | _ ||- y ≅ y' : _])
-  (RIAxy : [Γ ||-<l> tId A x y])
+  (RIAxy : [Γ ||-<l> tId A x y ≅ tId A' x' y'])
   (Ree' : [RIAxy | _ ||- e ≅ e' : _])
   (Pee' : IdPropEq (normRedId RIAxy) e e') :
   [RP Ryy' Ree' | _ ||- tIdElim A x P hr y e ≅ tIdElim A' x' P' hr' y' e' : _].
 Proof.
   pose proof (RP _ _ _ _ Rxx' _ Rrfl).
   pose proof (RP _ _ _ _ Ryy' _ Ree').
-  destruct Pee'; cbn in *; escape.
+  destruct Pee' as [B B' z z' ?????? xz xz' yz yz'|]; cbn in *; escape.
   - eapply redSubstTmEq; cycle 1.
     + eapply redtm_idElimRefl; tea.
-      transitivity x'0; [|symmetry]; tea.
+      transitivity z; [|symmetry]; tea.
     + eapply redtm_idElimRefl; tea.
       1-4: eapply ty_conv; tea.
       1: transitivity A; tea; now symmetry.
       2: eapply convtm_conv; [transitivity x; tea; now symmetry|tea].
       eapply convtm_conv; [transitivity y; tea|tea].
-      transitivity x0; symmetry; tea.
+      transitivity z; symmetry; tea.
       transitivity x; tea; now symmetry.
-    + eapply irrLRConv; tea.
-      etransitivity; [|symmetry]; eapply RP.
-      4: now eapply lrefl.
-      1,3: eapply irrLR; first [eapply e| eapply e1].
-      eapply reflCongRed; tea.
-      Unshelve. tea.
+    + assert [RA | _ ||- x ≅ y' : _].
+      1: transitivity y; tea; transitivity z; [|symmetry]; now eapply irrLR.
+      eapply irrLRConv; tea.
+      unshelve (etransitivity; [|symmetry]; eapply RP; cycle 3; tea).
+      1: now eapply IdRed.
+      now eapply reflCongRed0.
   - eapply reflectLR.
     + now eapply ty_IdElim.
     + eapply ty_conv; [|symmetry; tea].
       eapply ty_IdElim; tea.
       all: eapply ty_conv; tea.
-      now eapply convty_Id.
     + eapply convneu_IdElim; tea.
       destruct r;  now cbn in *.
 Qed.
 
 
 Lemma idElimCongRed {Γ l A A' x x' P P' hr hr' y y' e e'}
-  (RA : [Γ ||-<l> A])
-  (RA' : [Γ ||-<l> A'])
-  (wtyA' := escape RA')
-  (convtyAA' : [Γ |- A ≅ A' ])
+  (RA : [Γ ||-<l> A ≅ A'])
   (Rxx' : [RA | _ ||- x ≅ x' : _])
-  (RIAxx : [Γ ||-<l> tId A x x])
+  (RIAxx : [Γ ||-<l> tId A x x ≅ tId A' x' x'])
   (RP0 : [Γ ,, A ,, tId A⟨@wk1 Γ A⟩ x⟨@wk1 Γ A⟩ (tRel 0) |- P])
   (RP0' : [Γ ,, A' ,, tId A'⟨@wk1 Γ A'⟩ x'⟨@wk1 Γ A'⟩ (tRel 0) |- P'])
   (RPP0 : [Γ ,, A ,, tId A⟨@wk1 Γ A⟩ x⟨@wk1 Γ A⟩ (tRel 0) |- P ≅ P'])
   (RP : forall {y y' e e'}
     (Ryy' : [RA | _ ||- y ≅ y' : _])
-    {RIAxy : [Γ ||-<l> tId A x y]}
+    {RIAxy : [Γ ||-<l> tId A x y ≅ tId A' x' y']}
     (Ree' : [ RIAxy | _ ||- e ≅ e' : _]),
     [Γ ||-<l> P[e .: y..] ≅ P'[e' .: y'..]])
-  (Rrfl := (reflCongRed RA wtyA' convtyAA' Rxx' RIAxx))
+  (Rrfl := (reflCongRed RA Rxx' RIAxx))
   (Rhrhr' : [RP Rxx' Rrfl | _ ||- hr ≅ hr' : _])
   (Ryy' : [RA | _ ||- y ≅ y' : _])
-  (RIAxy : [Γ ||-<l> tId A x y])
+  (RIAxy : [Γ ||-<l> tId A x y ≅ tId A' x' y'])
   (Ree' : [RIAxy | _ ||- e ≅ e' : _]) :
   [RP Ryy' Ree' | _ ||- tIdElim A x P hr y e ≅ tIdElim A' x' P' hr' y' e' : _].
 Proof.
@@ -232,8 +165,8 @@ Proof.
   pose proof (redTmFwd' nRee') as [].
   eapply redSubstTmEq.
   + eapply irrLRConv.
-    2: unshelve (eapply idElimPropCongRed; cycle 3; tea; exact (nRee'.(IdRedTmEq.prop)));
-     [|tea|now eapply irrLR].
+    2: unshelve (eapply idElimPropCongRed; cycle 4; [exact (nRee'.(IdRedTmEq.prop))| tea..]); tea.
+    2: now eapply irrLR.
     etransitivity; [|symmetry]; eapply RP; cycle 1; [now eapply lrefl| tea..].
   + escape; eapply redtm_idElim; tea; eapply tmr_wf_red; exact (whredtmL nRee').(tmred_whnf_red).
   + escape; eapply redtm_idElim; tea.
@@ -242,7 +175,6 @@ Proof.
     2: unfold IdRedTy.outTy; cbn; gtyping.
     eapply ty_conv; tea; eapply escapeEq, RP; tea.
 Qed.
-
 
 
 
